Implement thm_to_string

candle/standard/ml_kernel/candle_kernelProgScript.sml
@@ -3,9 +3,12 @@
 *)
 open preamble;
 open ml_translatorLib ml_monad_translatorLib ml_progLib ml_hol_kernel_funsProgTheory;
-open basisFunctionsLib;
+open basisFunctionsLib print_thmTheory;
+open (* lisp: *) lisp_parsingTheory lisp_valuesTheory lisp_printingTheory;
 
 val _ = new_theory "candle_kernelProg";
+
+val _ = set_grammar_ancestry ["ml_hol_kernel_funsProg"];
 
 val _ = m_translation_extends "ml_hol_kernel_funsProg"
 
@@ -13,11 +16,48 @@ val _ = (use_long_names := false);
 
 val _ = ml_prog_update open_local_block;
 
-Definition thm_to_string_def:
-  thm_to_string (ctxt:update list) (th:thm) = strlit "thm here!"
-End
+val r = translate lisp_valuesTheory.name_def;
+val r = translate lisp_printingTheory.num2ascii_def;
+val r = translate lisp_printingTheory.ascii_name_def;
 
-val _ = translate thm_to_string_def;
+val lemma = prove(“ascii_name_side v3”,
+  fs [fetch "-" "ascii_name_side_def"]
+  \\ fs [Once lisp_printingTheory.num2ascii_def,AllCaseEqs()])
+  |> update_precondition;
+
+val r = translate num2str_def;
+
+val lemma = prove(“∀n. num2str_side n”,
+  ho_match_mp_tac lisp_printingTheory.num2str_ind
+  \\ rw [] \\ simp [Once (fetch "-" "num2str_side_def")]
+  \\ rw [] \\ gvs [DIV_LT_X]
+  \\ ‘n MOD 10 < 10’ by fs []
+  \\ decide_tac)
+  |> update_precondition;
+
+val r = translate lisp_printingTheory.name2str_def;
+val r = translate lisp_valuesTheory.list_def;
+val r = translate nil_list_def;
+val r = translate str_to_v_def;
+val r = translate ty_to_v_def;
+val r = translate term_to_v_def;
+val r = translate thm_to_v_def;
+val r = translate update_to_v_def;
+val r = translate dest_quote_def;
+val r = translate dest_list_def;
+val r = translate newlines_def;
+val r = translate v2pretty_def;
+val r = translate get_size_def;
+val r = translate get_next_size_def;
+val r = translate annotate_def;
+val r = translate remove_all_def;
+val r = translate smart_remove_def;
+val r = translate flatten_def;
+val r = translate dropWhile_def;
+val r = translate is_comment_def;
+val r = translate v2str_def;
+val r = translate vs2str_def;
+val r = translate thm_to_string_def;
 
 val _ = ml_prog_update open_local_in_block;
 
